Interface.v
@@ -2,291 +2,63 @@ Require Import lib.Integers.
 Require Import lib.Floats.
 Require Import Rustre.Common.
 
+Require compcert.common.Values.
+Require compcert.cfrontend.Cop.
+Require compcert.cfrontend.Ctypes.
+Require compcert.common.Memory.
+Require compcert.lib.Maps.
+
 (* Interface avec CompCert *)
-Inductive val'': Type :=
-(* | Vundef: val'' *)
-| Vint: Int.int -> val''
-| Vfloat: float32 -> val''.
 
-Inductive typ': Type :=
-| Tbool
-| Tvoid
-| Tint
-| Tfloat.
-
-Inductive unary_op': Type :=
-| Opposite
-| Negation.
-
-Inductive binary_op': Type :=
-| Add
-| Sub
-| Mul
-| Div.
-
-Definition zero := Int.zero.
-Definition one := Int.one.
+Definition empty_composite_env : Ctypes.composite_env := (Maps.PTree.empty _).
 
 Module Export Op <: OPERATORS.
-  Definition val': Type := val''.
-              
-  Inductive val: Type :=
-  | Vbool: bool -> val
-  | Val: val' -> val.
+  Definition val: Type := Values.val.
 
-  Definition Vzero := Val (Vint Int.zero).
+  (* TODO: wrong! Fix. *)
+  Definition typ := Ctypes.type.
 
-  Definition typ := typ'.
+  Definition true_val := Values.Vtrue.
+  Definition false_val := Values.Vfalse.
 
+  Lemma true_not_false_val: true_val <> false_val.
+  Proof. discriminate. Qed.
+
+  (* Wrong. TODO: Fix this. *)
   Definition typ_of_val (v: val): typ :=
     match v with
-    | Vbool _ => Tbool
-    | Val v =>
-      match v with
-      (* | Vundef => Tvoid *)
-      | Vint _ => Tint
-      | Vfloat _ => Tfloat
-      end
+    (* | Vundef => Tvoid *)
+    | Values.Vint _ => Ctypes.Tvoid
+    | Values.Vfloat _ => Ctypes.Tvoid
+    | _ => Ctypes.Tvoid
     end.
     
-  Definition unary_op := unary_op'.
-  Definition binary_op := binary_op'.
+  Definition unary_op := Cop.unary_operation.
+  Definition binary_op := Cop.binary_operation.
 
-  Definition opt (v: val'): option val := Some (Val v).
-  
-  Definition of_bool (b: bool): val' := Vint (if b then one else zero).
+  Definition sem_unary (op: unary_op) (v: val) (ty: typ) : option val :=
+    Cop.sem_unary_operation op v ty Memory.Mem.empty.
 
-  Definition sem_val_unary (sem: val' -> typ -> option val) (v: val): typ -> option val :=
-    match v with
-    | Vbool b => sem (of_bool b)   
-    | Val v => sem v
-    end.
-  
-  Definition sem_opposite: val -> typ -> option val :=
-    let sem v ty :=
-        match v, ty with
-        | Vint n, (Tint | Tbool) => opt (Vint (Int.neg n))
-        | Vfloat f, Tfloat => opt (Vfloat (Float32.neg f))
-        | _, _ => None
-        end
-    in sem_val_unary sem.
-  
-  Definition sem_negation: val -> typ -> option val :=
-    let sem v ty :=
-        match v, ty with
-        | Vint n, (Tint | Tbool) => opt (of_bool (Int.eq n zero))
-        | Vfloat f, Tfloat => opt (of_bool (Float32.cmp Ceq f Float32.zero))
-        | _, _ => None
-        end
-    in sem_val_unary sem.
-    
-  Definition sem_unary (op: unary_op): val -> typ -> option val :=
-    match op with
-    | Opposite => sem_opposite 
-    | Negation => sem_negation 
-    end.
+  Definition sem_binary (op: binary_op)
+             (v1: val) (ty1: typ)
+             (v2: val) (ty2: typ) : option val :=
+    Cop.sem_binary_operation
+      empty_composite_env op v1 ty1 v2 ty2 Memory.Mem.empty.
 
-  Inductive classify_cast_cases :=
-  | cast_case_neutral
-  | cast_case_f2bool
-  | cast_case_i2bool
-  | cast_case_f2i
-  | cast_case_f2f
-  | cast_case_i2f
-  | cast_case_void
-  | cast_case_default.
-  
-  Definition classify_cast (tfrom tto: typ) : classify_cast_cases :=
-    match tto, tfrom with
-    | Tint, (Tint | Tbool) => cast_case_neutral
-    | Tbool, Tfloat => cast_case_f2bool
-    | Tbool, Tint => cast_case_i2bool
-    | Tint, Tfloat => cast_case_f2i
-    | Tfloat, Tfloat => cast_case_f2f
-    | Tfloat, (Tint | Tbool) => cast_case_i2f 
-    | Tvoid, _ => cast_case_void
-    | _, _ => cast_case_default
-    end.
+  Lemma val_dec   : forall v1 v2 : val, {v1 = v2} + {v1 <> v2}.
+  Proof Values.Val.eq.
 
-  Definition sem_cast (v: val') (ty1 ty2: typ) : option val' :=
-    match classify_cast ty1 ty2 with
-    | cast_case_neutral =>
-      match v with
-      | Vint _ => Some v
-      | _ => None
-      end
-    | cast_case_f2bool =>
-      match v with
-      | Vfloat f => Some (of_bool (Float32.cmp Ceq f Float32.zero))
-      | _ => None
-      end
-    | cast_case_i2bool =>
-      match v with
-      | Vint i => Some (of_bool (Int.eq i Int.zero))
-      | _ => None
-      end
-    | cast_case_f2i =>
-      match v with
-      | Vfloat f =>
-        match Float32.to_int f with
-        | Some i => Some (Vint i)
-        | None => None
-        end
-      | _ => None
-      end
-    | cast_case_f2f =>
-      match v with
-      | Vfloat f => Some (Vfloat f)
-      | _ => None
-      end
-    | cast_case_i2f =>
-      match v with
-      | Vint i => Some (Vfloat (Float32.of_int i))
-      | _ => None
-      end
-    | cast_case_void => Some v
-    | cast_case_default => None
-    end.
-
-  Definition binarith_type (ty1 ty2: typ) : typ :=
-    match ty1, ty2 with
-    | (Tint | Tbool), (Tint | Tbool) => Tint
-    | Tfloat, Tfloat
-    | (Tint | Tbool), Tfloat
-    | Tfloat, (Tint | Tbool) => Tfloat
-    | _, _ => Tvoid
-    end.
-
-  Definition sem_binarith
-    (sem_int: int -> int -> option val)
-    (sem_float: float32 -> float32 -> option val)
-    (v1 v2: val') (ty1 ty2: typ): option val :=
-    let ty := binarith_type ty1 ty2 in
-    match sem_cast v1 ty1 ty with
-    | None => None
-    | Some v1' =>
-      match sem_cast v2 ty2 ty with
-      | None => None
-      | Some v2' =>
-        match ty with
-        | Tint =>
-          match v1', v2' with
-          | Vint n1, Vint n2 => sem_int n1 n2
-          | _, _ => None
-          end
-        | Tfloat =>
-          match v1', v2' with
-          | Vfloat f1, Vfloat f2 => sem_float f1 f2
-          | _, _ => None
-          end
-        | bin_default => None
-        end
-      end
-    end.
-  
-  Definition sem_val_binary (sem: val' -> val' -> typ -> typ -> option val) (v1 v2: val)
-    : typ -> typ -> option val :=
-    match v1, v2 with
-    | Vbool b1, Vbool b2 => sem (of_bool b1) (of_bool b2)
-    | Val v1, Vbool b2 => sem v1 (of_bool b2)
-    | Vbool b1, Val v2 => sem (of_bool b1) v2
-    | Val v1, Val v2 => sem v1 v2
-    end.
-  
-  Definition sem_add: val -> val -> typ -> typ -> option val :=
-    let sem_int n1 n2 := opt (Vint (Int.add n1 n2)) in
-    let sem_float f1 f2 := opt (Vfloat (Float32.add f1 f2)) in
-    sem_val_binary (sem_binarith sem_int sem_float).
-
-  Definition sem_sub: val -> val -> typ -> typ -> option val :=
-    let sem_int n1 n2 := opt (Vint (Int.sub n1 n2)) in
-    let sem_float f1 f2 := opt (Vfloat (Float32.sub f1 f2)) in
-    sem_val_binary (sem_binarith sem_int sem_float).
-
-  Definition sem_mul: val -> val -> typ -> typ -> option val :=
-    let sem_int n1 n2 := opt (Vint (Int.mul n1 n2)) in
-    let sem_float f1 f2 := opt (Vfloat (Float32.mul f1 f2)) in
-    sem_val_binary (sem_binarith sem_int sem_float).
-
-  Definition sem_div: val -> val -> typ -> typ -> option val :=
-    let sem_int n1 n2 :=
-        if Int.eq n2 Int.zero
-           || Int.eq n1 (Int.repr Int.min_signed) && Int.eq n2 Int.mone
-        then None else opt (Vint (Int.divs n1 n2))
-    in
-    let sem_float f1 f2 := opt (Vfloat (Float32.div f1 f2)) in
-    sem_val_binary (sem_binarith sem_int sem_float).
-  
-  Definition sem_binary (op: binary_op) (v1: val) (ty1: typ) (v2: val) (ty2: typ): option val :=
-    (match op with
-    | Add => sem_add
-    | Sub => sem_sub
-    | Mul => sem_mul
-    | Div => sem_div
-    end) v1 v2 ty1 ty2.
-    
-  (* Lemma val_dec: forall v1 v2: val, {v1 = v2} + {v1 <> v2}. *)
-  (* Proof. *)
-  (*   decide equality. *)
-  (*   apply Bool.bool_dec. *)
-  (*   decide equality. *)
-  (*   apply Int.eq_dec. *)
-  (*   apply Float.eq_dec. *)
-  (* Qed. *)
-
-  Definition val_eqb (v1 v2: val): bool :=
-    match v1, v2 with
-    | Vbool b1, Vbool b2 => Bool.eqb b1 b2
-    | Val v1, Val v2 =>
-      match v1, v2 with
-      (* | Vundef, Vundef => true *)
-      | Vint n1, Vint n2 => Int.eq n1 n2
-      | Vfloat f1, Vfloat f2 => if Float32.eq_dec f1 f2 then true else false
-      | _, _ => false
-      end
-    | _, _ => false
-    end.
-
-  Definition typ_eqb (ty1 ty2: typ): bool :=
-    match ty1, ty2 with
-    | Tbool, Tbool
-    | Tvoid, Tvoid
-    | Tint, Tint
-    | Tfloat, Tfloat => true
-    | _, _ => false
-    end.
-  
-  Lemma unop_dec: forall op1 op2: unary_op, {op1 = op2} + {op1 <> op2}.
-  Proof. decide equality. Qed.
-  Definition unop_eqb (op1 op2: unary_op) := if unop_dec op1 op2 then true else false.
-
-  Lemma binop_dec: forall op1 op2: binary_op, {op1 = op2} + {op1 <> op2}.
-  Proof. decide equality. Qed.
-  Definition binop_eqb (op1 op2: binary_op) := if binop_dec op1 op2 then true else false.
-  
-  Theorem val_eqb_iff: forall v1 v2, val_eqb v1 v2 = true <-> v1 = v2.
+  Lemma typ_dec   : forall t1 t2 : typ, {t1 = t2} + {t1 <> t2}.
+  Proof Ctypes.type_eq.
+      
+  Lemma unop_dec  : forall op1 op2 : unary_op, {op1 = op2} + {op1 <> op2}.
   Proof.
-    intros v1 v2; unfold val_eqb; destruct v1 as [b1|v1], v2 as [b2|v2];
-    try destruct b1, b2; try destruct v1 as [n1|f1], v2 as [n2|f2];
-    try intuition discriminate.
-    - split; intro H.
-      + pose proof (Int.eq_spec n1 n2) as Heq; rewrite H in Heq; now do 2 f_equal.
-      + inversion H; apply Int.eq_true.
-    - split; intro H.
-      + destruct (Float32.eq_dec f1 f2).
-        * now inversion e.
-        * discriminate.
-      + destruct (Float32.eq_dec f1 f2); auto.
-        exfalso; apply n; now inversion H.
+    decide equality.
   Qed.
 
-  Theorem typ_eqb_iff : forall t1 t2, typ_eqb t1 t2 = true <-> t1 = t2.
-  Proof. intros ty1 ty2; destruct ty1, ty2; intuition discriminate. Qed.
-
-  Theorem unop_eqb_iff: forall op1 op2, unop_eqb op1 op2 = true <-> op1 = op2.
-  Proof. intros op1 op2; unfold unop_eqb; destruct (unop_dec op1 op2); intuition discriminate. Qed.
-  
-  Theorem binop_eqb_iff: forall op1 op2, binop_eqb op1 op2 = true <-> op1 = op2. 
-  Proof. intros op1 op2; unfold binop_eqb; destruct (binop_dec op1 op2); intuition discriminate. Qed.
-  
+  Lemma binop_dec : forall op1 op2 : binary_op, {op1 = op2} + {op1 <> op2}.
+  Proof.
+    decide equality.
+  Qed.
+    
 End Op.
