Minimp.v
@@ -4,8 +4,8 @@ Require Export Minimp.Equiv.
 
 Require Import Rustre.Common.
 
-Module Type MINIMP (Op: OPERATORS).
-  Declare Module Export Syn: SYNTAX Op.
-  Declare Module Export Sem: SEMANTICS Op Syn.
-  Declare Module Export Equ: EQUIV Op Syn Sem.
+Module Type MINIMP (Op: OPERATORS) (OpAux: OPERATORS_AUX Op).
+  Declare Module Export Syn: SYNTAX Op OpAux.
+  Declare Module Export Sem: SEMANTICS Op OpAux Syn.
+  Declare Module Export Equ: EQUIV Op OpAux Syn Sem.
 End MINIMP.
