Minimp/Syntax.v
@@ -14,7 +14,9 @@ Open Scope list_scope.
   two methods: [step] and [reset].
 
  *)
-Module Type PRE_SYNTAX (Import Op : OPERATORS).
+Module Type PRE_SYNTAX
+       (Import Op : OPERATORS)
+       (Import OpAux : OPERATORS_AUX Op).
 
   Inductive exp : Type :=
   | Var : ident -> typ -> exp                    (* variable  *)
@@ -75,9 +77,11 @@ Module Type PRE_SYNTAX (Import Op : OPERATORS).
 
 End PRE_SYNTAX.
 
-Module Type SYNTAX (Import Op : OPERATORS).
+Module Type SYNTAX
+       (Import Op : OPERATORS)
+       (Import OpAux : OPERATORS_AUX Op).
 
-  Include PRE_SYNTAX Op.
+  Include PRE_SYNTAX Op OpAux.
 
   (** ** Decidable equality *)
 
@@ -88,8 +92,10 @@ Module Type SYNTAX (Import Op : OPERATORS).
 
 End SYNTAX.
 
-Module SyntaxFun (Import Op : OPERATORS) <: SYNTAX Op.
-  Include PRE_SYNTAX Op.
+Module SyntaxFun
+       (Import Op : OPERATORS)
+       (Import OpAux : OPERATORS_AUX Op) <: SYNTAX Op OpAux.
+  Include PRE_SYNTAX Op OpAux.
 
   Implicit Type e: exp.
   Implicit Type s: stmt.
@@ -123,12 +129,15 @@ Module SyntaxFun (Import Op : OPERATORS) <: SYNTAX Op.
     fix 1.
     intros e1 e2.
     refine (match e1, e2 with
-            | Var x1 ty1, Var x2 ty2 => ident_eqb x1 x2 && typ_eqb ty1 ty2
-            | State s1 ty1, State s2 ty2 => ident_eqb s1 s2 && typ_eqb ty1 ty2
-            | Const c1 ty1, Const c2 ty2 => val_eqb c1 c2 && typ_eqb ty1 ty2
+            | Var x1 ty1, Var x2 ty2 => ident_eqb x1 x2 && equiv_decb ty1 ty2
+            | State s1 ty1, State s2 ty2 => ident_eqb s1 s2 && equiv_decb ty1 ty2
+            | Const c1 ty1, Const c2 ty2 => equiv_decb c1 c2 && equiv_decb ty1 ty2
             (* | Op op1 es1, Op op2 es2 => op_eqb op1 op2 && _ *)
-            | Unop op1 e1' ty1, Unop op2 e2' ty2 => unop_eqb op1 op2  && typ_eqb ty1 ty2 && _
-            | Binop op1 e11 e12 ty1, Binop op2 e21 e22 ty2 => binop_eqb op1 op2  && typ_eqb ty1 ty2 && _
+            | Unop op1 e1' ty1, Unop op2 e2' ty2 => equiv_decb op1 op2
+                                                 && equiv_decb ty1 ty2 && _
+            | Binop op1 e11 e12 ty1, Binop op2 e21 e22 ty2 => equiv_decb op1 op2
+                                                           && equiv_decb ty1 ty2
+                                                           && _
             | _, _ => false
             end).
     - exact (exp_eqb e1' e2').
@@ -145,13 +154,13 @@ Module SyntaxFun (Import Op : OPERATORS) <: SYNTAX Op.
       exp_eqb e1 e2 = true <-> e1 = e2.
   Proof.
     induction e1 (* using exp_ind2 *); intros e2; destruct e2; simpl; try now split; intro; discriminate.
-    - rewrite Bool.andb_true_iff, ident_eqb_eq, typ_eqb_iff.
+    - rewrite Bool.andb_true_iff, ident_eqb_eq, equiv_decb_equiv.
       split; intro Heq; [now f_equal | now inversion Heq].
-    - rewrite Bool.andb_true_iff, ident_eqb_eq, typ_eqb_iff.
+    - rewrite Bool.andb_true_iff, ident_eqb_eq, equiv_decb_equiv.
       split; intro Heq; [now f_equal | now inversion Heq].
-    - rewrite Bool.andb_true_iff, typ_eqb_iff, val_eqb_iff.
+    - rewrite Bool.andb_true_iff, equiv_decb_equiv, equiv_decb_equiv.
       split; intro Heq; [now f_equal | now inversion Heq].
-    - rewrite 2 Bool.andb_true_iff, typ_eqb_iff, unop_eqb_iff.
+    - rewrite 2 Bool.andb_true_iff, equiv_decb_equiv, equiv_decb_equiv.
       split; intro Heq.
       + f_equal; try apply IHe1; apply Heq.
       (* auto. destruct Heq as [? Heq]; subst; split || f_equal; trivial; []. *)
@@ -164,7 +173,7 @@ Module SyntaxFun (Import Op : OPERATORS) <: SYNTAX Op.
       + now inversion Heq; subst; rewrite IHe1. (* trivial. split; trivial. clear Heq. induction n; simpl; [|]. *)
     (* * inversion_clear IHes. now rewrite H. *)
     (* * inversion_clear IHes. rewrite Bool.andb_true_iff, H. split; trivial. now apply IHn. *)
-    - rewrite 3 Bool.andb_true_iff, typ_eqb_iff, binop_eqb_iff.
+    - rewrite 3 Bool.andb_true_iff, equiv_decb_equiv, equiv_decb_equiv.
       rewrite IHe1_1, IHe1_2.
       split; intro Heq.
       + f_equal; apply Heq.
